Runtime/SortedArray.lean
@@ -13,6 +13,14 @@ namespace SortedArray
 
 variable [Ord α]
 
+def coe [Ord β] [Coe α β] (s : SortedArray α) (h : ∀ a₁ a₂, compare a₁ a₂ = compare (a₁ : β) (a₂ : β)) : SortedArray β := {
+  toArray := s.toArray.map Coe.coe
+  isSorted := sorry
+}
+
+instance [Ord β] [ordCoe : OrdCoe α β] : Coe (SortedArray α) (SortedArray β) where
+  coe s := s.coe ordCoe.coeOrd
+
 def nil : SortedArray α := {
   isSorted := List.Sorted.nil
 }
@@ -25,12 +33,36 @@ def singleton (a : α) : SortedArray α := {
 
 notation (priority := default - 1) "#[" a "]#" => SortedArray.singleton a
 
+instance : LE (SortedArray α) where
+  le s₁ s₂ := 
+    match s₁.toArray[s₁.size - 1]?, s₂.toArray[0]? with
+    | _, none | none, _ => True
+    | some last₁, some first₂ => last₁ ≤ first₂
+
+def append (s₁ s₂ : SortedArray α) (h : s₁ ≤ s₂) : SortedArray α :=
+  ⟨s₁.toArray ++ s₂.toArray, sorry⟩ 
+
+-- Note: For the purposes of reactor execution, it is important that this merge is stable
+--       in the sense that for elements of equal ordering, those from s₁ are sorted earlier 
+--       than those from s₂. Also the order present within a given array (s₁ or s₂) is not 
+--       disturbed.
 def merge (s₁ s₂ : SortedArray α) : SortedArray α :=
-  go 0 0 s₁ s₂ #[]#
-where 
-  go (i₁ i₂ : Nat) (s₁ s₂ acc : SortedArray α) (h₁ : i₁ ≤ s₁.size := by simp) (h₂ : i₂ ≤ s₂.size := by simp) : SortedArray α :=
-  -- TODO: temporary - This will only work if the sort is stable!
+  -- TODO: temporary
   let sorted := (s₁.toArray ++ s₂.toArray).insertionSort (Ord.compare · · |>.isLE)
   { toArray := sorted, isSorted := sorry }
+  
+-- Note: For the purposes of reactor execution, it is important that this split is stable.
+def split (s : SortedArray α) (p : α → Bool) : (SortedArray α) × (SortedArray α) :=
+  -- TODO: temporary - This can be done more efficiently (note: Array.split is stable)
+  let ⟨fst, snd⟩ := s.toArray.split p
+  (⟨fst, sorry⟩, ⟨snd, sorry⟩)
 
+def unique (s : SortedArray α) (f : α → β) [DecidableEq β] : (SortedArray α) × (SortedArray α) := Id.run do
+  let mut included : Array α := #[] 
+  let mut excluded : Array α := #[]
+  for a in s.toArray do
+    if included.any (f a = f ·) 
+    then excluded := excluded.push a
+    else included := included.push a
+  return (⟨included, sorry⟩, ⟨excluded, sorry⟩)
   
