Runtime/Time.lean
@@ -5,16 +5,42 @@ abbrev Time.From (time : Time) := { t : Time // t ≥ time }
 instance : Ord (Time.From time) where
   compare t₁ t₂ := compare t₁.val t₂.val
 
+def Time.From.lift (t : Time.From later) (h : later ≥ earlier) : Time.From earlier := {
+  val := t
+  property := Nat.le_trans h t.property
+}
+
+instance {later : Time.From earlier} : Coe (Time.From later) (Time.From earlier) where
+  coe t := t.lift later.property
+
 structure Tag where
   time : Time
   microstep : Nat
+
+abbrev Tag.From (time : Time) := { tag : Tag // tag.time ≥ time }
+
+def Tag.From.time {time : Time} (tag : Tag.From time) : Time.From time := { 
+  val := tag.val.time
+  property := tag.property
+}
+
+def Tag.From.lift (t : Tag.From later) (h : later ≥ earlier) : Tag.From earlier := {
+  val := t
+  property := Nat.le_trans h t.property
+}
+
+instance {later : Time.From earlier} : Coe (Tag.From later) (Tag.From earlier) where
+  coe t := t.lift later.property
 
 def Time.advance (time : Time) (d : Duration) : Time.From time := {
   val := time + d
   property := by simp_arith
 }
 
-def Tag.advance (tag : Tag) (time : Time.From tag.time) : Tag := {
-  time := time
-  microstep := if tag.time = time then tag.microstep + 1 else 0
+def Tag.advance (tag : Tag) (time : Time.From tag.time) : Tag.From time := {
+  val := {
+    time := time
+    microstep := if tag.time = time then tag.microstep + 1 else 0
+  }
+  property := by simp
 }
